Types/Expr/Repl.lean
@@ -1,4 +1,5 @@
 import Types.Expr.Stx
+import Types.Expr.TRepl
 
 namespace Expr
 
@@ -7,14 +8,14 @@ def bvarShift (shift skip : Nat) : Expr → Expr
   | .app a b => .app (a.bvarShift shift skip) (b.bvarShift shift skip)
   | .lam ty body => .lam ty (body.bvarShift shift skip.succ)
   | .tapp expr ty => .tapp (expr.bvarShift shift skip) ty
-  | .tlam body => .tlam (body.bvarShift shift skip.succ)
+  | .tlam body => .tlam (body.bvarShift shift skip)
 
 def bvarUnShift (shift skip : Nat) : Expr → Expr
   | .id n => .id $ if n - shift < skip then n else n - shift
   | .app a b => .app (a.bvarUnShift shift skip) (b.bvarUnShift shift skip)
   | .lam ty body => .lam ty (body.bvarUnShift shift skip.succ)
   | .tapp expr ty => .tapp (expr.bvarUnShift shift skip) ty
-  | .tlam body => .tlam (body.bvarUnShift shift skip.succ)
+  | .tlam body => .tlam (body.bvarUnShift shift skip)
 
 def replace.bvar (bvarId idx_shift : Nat) (replace : Expr) : Expr :=
   match compare bvarId idx_shift with
@@ -23,13 +24,13 @@ def replace.bvar (bvarId idx_shift : Nat) (replace : Expr) : Expr :=
   | .gt => .id bvarId.pred
 
 -- Replace also needs to add idx to every value within replace to ensure that the binders still point towards the right points
-def replace (idx_shift : Nat) (body replace : Expr) : Expr := match body with
-  | .id n => Expr.replace.bvar n idx_shift replace
-  | .app a b => .app (a.replace idx_shift replace) (b.replace idx_shift replace)
-  | .lam ty body => .lam ty (body.replace idx_shift.succ replace)
-  | .tapp expr ty => .tapp (expr.replace idx_shift replace) ty
-  | .tlam body => .tlam (body.replace idx_shift.succ replace)
+def replace (idx_shift tshift : Nat) (body replace : Expr) : Expr := match body with
+  | .id n => Expr.replace.bvar n idx_shift (replace.tBvarShift tshift 0)
+  | .app a b => .app (a.replace idx_shift tshift replace) (b.replace idx_shift tshift replace)
+  | .lam ty body => .lam ty (body.replace idx_shift.succ tshift replace)
+  | .tapp expr ty => .tapp (expr.replace idx_shift tshift replace) ty
+  | .tlam body => .tlam (body.replace idx_shift tshift.succ replace)
 
-def β (body repl : Expr) : Expr := (body.replace 0 repl)
+def β (body repl : Expr) : Expr := (body.replace 0 0 repl)
 
 end Expr
