Types/BLang.lean
@@ -1,0 +1,103 @@
+
+namespace BLang
+
+inductive Ty
+  | bool
+  | int
+
+def Ty.denote : Ty → Type
+  | .bool => Prop
+  | .int => Int
+
+namespace BLang1
+
+inductive Stx : Ty → Type
+  | true : Stx .bool
+  | false : Stx .bool
+  | n (x : Nat) : Stx .int
+  | lt : Stx .int → Stx .int → Stx .bool
+  | add : Stx .int → Stx .int → Stx .int
+  | and : Stx .bool → Stx .bool → Stx .bool
+  | neg : Stx .bool → Stx .bool
+
+def Stx.denote : {t : Ty} → Stx t → t.denote
+  | .bool, .true => True
+  | .bool, .false => False
+  | .int, .n x => Int.ofNat x
+  | .bool, .lt a b => Int.lt (a.denote : Int) (b.denote : Int)
+  | .int, .add a b => Int.add a.denote b.denote
+  | .bool, .and a b => a.denote ∧ b.denote
+  | .bool, .neg a => ¬a.denote
+
+end BLang1
+
+def Ctx.denote (Γ : List Ty) : Type :=
+  (v : Fin Γ.length) → (Γ[v]).denote
+
+instance : Inhabited (Ctx.denote []) where
+  default x := x.elim0
+
+namespace BLang2
+
+inductive Stx : List Ty → Ty → Type
+  | true {Γ} : Stx Γ .bool
+  | false {Γ} : Stx Γ .bool
+  | n {Γ} (x : Nat) : Stx Γ .int
+  | lt {Γ} : Stx Γ .int → Stx Γ .int → Stx Γ .bool
+  | add {Γ} : Stx Γ .int → Stx Γ .int → Stx Γ .int
+  | and {Γ} : Stx Γ .bool → Stx Γ .bool → Stx Γ .bool
+  | neg {Γ} : Stx Γ .bool → Stx Γ .bool
+  | lete {Γ t t'} : Stx Γ t → Stx (t :: Γ) t' → Stx Γ t'
+  | var {Γ} (idx : Fin Γ.length) : Stx Γ Γ[idx]
+
+def Stx.denote {Γ} (γ : Ctx.denote Γ): {t : Ty} → Stx Γ t → t.denote
+  | _, .true => True
+  | _, .false => False
+  | _, .n x => Int.ofNat x
+  | _, .lt a b => Int.lt (a.denote γ) (b.denote γ)
+  | _, .add a b => Int.add (a.denote γ) (b.denote γ)
+  | _, .and a b => (a.denote γ) ∧ (b.denote γ)
+  | _, .neg a => ¬(a.denote γ)
+  | _, .lete val body => body.denote fun
+    | ⟨0, _⟩ => val.denote γ
+    | ⟨v+1, p⟩ => γ ⟨v, by grind⟩
+  | _, .var idx => γ idx
+
+/- declare_syntax_cat stx_blang2 -/
+
+/- syntax "true" : stx_blang2 -/
+/- syntax "false" : stx_blang2 -/
+/- syntax num : stx_blang2 -/
+/- syntax ident : stx_blang2 -/
+/- syntax "!(" term ")" : stx_blang2 -/
+/- syntax "(" stx_blang2 ")" : stx_blang2 -/
+/- syntax stx_blang2 "<" stx_blang2 : stx_blang2 -/
+/- syntax stx_blang2 "+" stx_blang2 : stx_blang2 -/
+/- syntax stx_blang2 "&&" stx_blang2 : stx_blang2 -/
+/- syntax "!" stx_blang2 : stx_blang2 -/
+/- syntax "let" ident "=" stx_blang2 "in" stx_blang2 : stx_blang2 -/
+
+/- syntax "[bl2!" "(" term ")" ident* "|" stx_blang2 "]" : term -/
+/- syntax "[bl2|" stx_blang2 "]" : term -/
+
+/- macro_rules -/
+/-   | `([bl2! ($_) | true ]) => `(Stx.true) -/
+/-   | `([bl2! ($_) | false ]) => `(Stx.false) -/
+/-   | `([bl2! ($_) | $v:num ]) => `(Stx.n $v) -/
+/-   | `([bl2! ($_) | $v:ident ]) => `($v) -/
+/-   | `([bl2! ($_) | !($t) ]) => `($t) -/
+/-   | `([bl2! ($Γ) | ($v) ]) => `([bl2! ($Γ) |$v]) -/
+/-   | `([bl2! ($Γ) | $a < $b ]) => `(Stx.lt [bl2! ($Γ) | $a] [bl2! ($Γ) | $b]) -/
+/-   | `([bl2! ($Γ) | $a + $b ]) => `(Stx.add [bl2! ($Γ) | $a] [bl2! ($Γ) | $b]) -/
+/-   | `([bl2! ($Γ) | $a && $b ]) => `(Stx.and [bl2! ($Γ) | $a] [bl2! ($Γ) | $b]) -/
+/-   | `([bl2! ($Γ) | ! $a ]) => `(Stx.neg [bl2! ($Γ) | $a]) -/
+/-   | `([bl2! ($Γ) | let $x = $val in $body ]) => `(Stx.lete [bl2! ($Γ) | $val] [bl2! ($Γ) $x | $body]) -/
+/-   | `([bl2! ($Γ) $h $ids*| $v:ident ]) => -/
+/-     if h.getId = v.getId then `(Stx.var ⟨0, by simp⟩) -/
+/-     else `([bl2! ($Γ) $ids* | $v:ident]) -/
+/-   | `([bl2| $v]) => `([bl2! ([]) | $v]) -/
+
+/- end BLang2 -/
+
+#eval (Stx.lete (Γ := []) (.n 00) (.add (.var ⟨0, by grind⟩) (.var ⟨0, by grind⟩))).denote default
+
